qed server.updateEpoch

src/program_proof/pav/server.v
@@ -6,9 +6,9 @@ From Perennial.program_proof Require Import std_proof.
 From iris.unstable.base_logic Require Import mono_list.
 From stdpp Require Import gmap.
 From Perennial.base_logic Require Import ghost_map.
-From Perennial.algebra Require Import ghost_map_pers.
 
 Module epochInfo.
+
 Record t :=
   mk {
     tree: gmap (list w8) (list w8);
@@ -20,6 +20,7 @@ Record t :=
 
 Section defs.
 Context `{!heapGS Σ, !pavG Σ}.
+
 Definition own ptr obj : iProp Σ :=
   ∃ ptr_tr sl_prevLink sl_dig sl_link sl_linkSig d0 d1 d2 d3,
   "Htr" ∷ own_Tree ptr_tr obj.(tree) ∗
@@ -39,10 +40,12 @@ Definition valid pk epoch γtree obj : iProp Σ :=
   "#Htree_dig" ∷ is_tree_dig obj.(tree) obj.(dig) ∗
   "#Hbind" ∷ is_hash (chainSepSome.encodesF (chainSepSome.mk epoch obj.(prevLink) obj.(dig))) obj.(link) ∗
   "#Hvalid_sig" ∷ is_sig pk (servSepLink.encodesF (servSepLink.mk obj.(link))) obj.(linkSig).
+
 End defs.
 End epochInfo.
 
 Module epochChain.
+
 Record t :=
   mk {
     epochs: list epochInfo.t;
@@ -50,6 +53,7 @@ Record t :=
 
 Section defs.
 Context `{!heapGS Σ, !pavG Σ}.
+
 Definition own ptr obj : iProp Σ :=
   ∃ sl_epochs ptr_epochs,
   "Hsl_epochs" ∷ own_slice_small sl_epochs ptrT (DfracOwn 1) ptr_epochs ∗
@@ -61,10 +65,31 @@ Definition valid pk γtrees obj : iProp Σ :=
   "#Hvalid_sep_chain" ∷ ([∗ list] k ↦ γtree; info ∈ γtrees; obj.(epochs),
     epochInfo.valid pk k γtree info) ∗
   "#Hbinds_chain" ∷ binds (epochInfo.dig <$> obj.(epochs)) (epochInfo.link <$> obj.(epochs)).
+
+Definition wp_put ptr_chain chain ptr_tree tree sl_sk pk γ γtrees γtree :
+  {{{
+    "Hown_chain" ∷ own ptr_chain chain ∗
+    "#Hvalid_chain" ∷ valid pk γtrees chain ∗
+    "Hown_tree" ∷ own_Tree ptr_tree tree ∗
+    "Hown_sk" ∷ own_sk sl_sk pk (serv_sigpred γ) ∗
+    "#Hpers_updates" ∷ ghost_map_auth_pers γtree tree
+  }}}
+  epochChain__put #ptr_chain #ptr_tree (slice_val sl_sk)
+  {{{
+    new_info, RET #();
+    let new_chain := mk (chain.(epochs) ++ [new_info]) in
+    "%Htr_witness" ∷ ⌜ new_info.(epochInfo.tree) = tree ⌝ ∗
+    "Hown_chain" ∷ own ptr_chain new_chain ∗
+    "#Hvalid_chain" ∷ valid pk (γtrees ++ [γtree]) new_chain ∗
+    "Hown_sk" ∷ own_sk sl_sk pk (serv_sigpred γ)
+  }}}.
+Proof. Admitted.
+
 End defs.
 End epochChain.
 
 Module server.
+
 Record t :=
   mk {
     mu: loc;
@@ -80,6 +105,8 @@ Definition own ptr obj : iProp Σ :=
   ∃ ptr_updates (updates : gmap (list w8) (list w8)) sl_updates ptr_chain γtrees γupdates chain,
   (* ghost state, the other half owned by global_inv. *)
   "HmonoTrees" ∷ mono_list_auth_own obj.(γ) (1/2) (γtrees ++ [γupdates]) ∗
+  (* need ghost_map_auth for next tr bc we're continuously updating it.
+  for older trees, epoch chain has ghost_map_auth_pers. *)
   "Hupdates_view" ∷ ghost_map_auth γupdates (1/2) updates ∗
 
   "Hown_sk" ∷ own_sk obj.(sl_sk) obj.(pk) (serv_sigpred obj.(γ)) ∗
@@ -90,8 +117,9 @@ Definition own ptr obj : iProp Σ :=
   "Hptr_chain" ∷ ptr ↦[server :: "chain"] #ptr_chain ∗
 
   (* exists (idS, sl_v) map that owns the respective (id, v) map. *)
-  "#Hsl_updates" ∷ ([∗ map] sl_v; v ∈ sl_updates; (kmap bytes_to_string updates),
-    own_slice_small sl_v byteT DfracDiscarded v) ∗
+  "#Hsl_updates" ∷ ([∗ map] id ↦ sl_v; v ∈ (kmap string_to_bytes sl_updates); updates,
+    "Hsl_v" ∷ own_slice_small sl_v byteT DfracDiscarded v ∗
+    "%Hlen_id" ∷ ⌜ length id = hash_len ⌝ ) ∗
   "Hown_updates" ∷ own_map ptr_updates (DfracOwn 1) sl_updates ∗
   "Hupdates" ∷ ptr ↦[server :: "updates"] #ptr_updates.
 
@@ -329,7 +357,6 @@ Lemma wp_applyUpdates ptr_currTr currTr (updates : gmap _ (list w8)) ptr_updates
 Proof.
   rewrite /applyUpdates.
   iIntros (Φ) "H HΦ"; iNamed "H".
-  wp_pures.
   wp_apply (wp_Tree_DeepCopy with "Hown_currTr");
     iEval (rewrite /named); iIntros (ptr_nextTr) "[Hown_currTr Hown_nextTr]".
   set (loopInv := λ (_ sl_mdone : gmap string Slice.t),
@@ -394,6 +421,7 @@ Proof.
   wp_loadField.
   wp_apply (acquire_spec with "[$HmuR]"); iIntros "[Hlocked Hown_serv]"; iNamed "Hown_serv".
 
+  (* index epochChain. *)
   wp_loadField.
   iNamed "Hown_chain".
   wp_loadField.
@@ -406,11 +434,60 @@ Proof.
     unshelve (epose proof (H _) as [ptr_epoch Hidx_ptr_epoch]);
     [word|]; clear H.
   wp_apply (wp_SliceGet with "[$Hsl_epochs //]"); iIntros "Hsl_epochs".
-  iDestruct (big_sepL2_lookup_1_some with "Hsep_epochs") as %[epoch_chain Hidx_epoch_chain]; [done|].
+  iDestruct (big_sepL2_lookup_1_some with "Hsep_epochs") as %[epoch_info Hidx_epoch_info]; [done|].
   iDestruct (big_sepL2_lookup_acc with "Hsep_epochs") as "[Hown_epoch Hsep_epochs]";
     [done..|]; iNamed "Hown_epoch".
   wp_loadField.
   wp_loadField.
-Admitted.
+  wp_apply (wp_applyUpdates with "[$Htr $Hown_updates $Hsl_updates]");
+    iIntros (ptr_nextTr); iNamed 1.
+  wp_loadField.
+  wp_loadField.
+  iDestruct ("Hsep_epochs" with
+    "[$Hsl_prevLink $Hsl_dig $Hsl_link $Hsl_linkSig $Hptr_tr $Hptr_prevLink $Hptr_dig
+    $Hptr_link $Hptr_linkSig $Hown_currTr]") as "Hown_epochs".
+
+  (* ghost_map_auth needs to match nextTr. *)
+  wp_apply ncfupd_wp.
+  iRename "HmonoTrees" into "HmonoTrees0".
+  iInv "Hinv" as "> H" "Hclose"; iNamed "H".
+  iDestruct (mono_list_auth_own_agree with "HmonoTrees HmonoTrees0") as %[_ ->].
+  iDestruct (big_sepL2_length with "Htree_views") as %Hlen0.
+  rewrite app_length in Hlen0.
+  list_simplifier.
+  unshelve (epose proof (list_snoc_exists trees _) as (old_trees & updates0 & ->)); [lia|].
+  (* we could do this with insert / delete, but snoc makes it easier to
+  unify the ghost state when closing the inv.
+  just pop the last off and push it back on. *)
+  iDestruct (big_sepL2_snoc with "Htree_views") as "[Htree_views Hupdates_view0]".
+  iDestruct (ghost_map_auth_agree with "Hupdates_view0 Hupdates_view") as %->.
+  iCombine "Hupdates_view Hupdates_view0" as "Hupdates_view".
+  iMod (ghost_map_apply_on epoch_info.(epochInfo.tree) with "Hupdates_view") as "[[Hauth_nextTr0 Hauth_nextTr] _]".
+  iDestruct (big_sepL2_snoc with "[$Htree_views $Hauth_nextTr0]") as "Htree_views".
+  (* also, make a new ghost_map since we're opening up a new epoch. *)
+  iMod ghost_map_alloc_empty as (γempty) "[Hauth_empty Hauth_empty0]".
+  iDestruct (big_sepL2_snoc with "[$Htree_views $Hauth_empty0]") as "Htree_views".
+  iCombine "HmonoTrees HmonoTrees0" as "HmonoTrees".
+  iMod (mono_list_auth_own_update_app [∅] with "HmonoTrees") as "[[HmonoTrees0 HmonoTrees] #Hmono_lb]".
+  iMod ("Hclose" with "[$HmonoTrees0 $Htree_views]") as "_".
+  iIntros "!>".
+
+  (* epochChain.put. *)
+  iMod (ghost_map_auth_persist with "Hauth_nextTr") as "#Hpers_nextTr".
+  wp_apply (epochChain.wp_put with
+    "[$Hown_epochs $Hown_nextTr $Hown_sk $Hsl_epochs $Hptr_epochs]");
+    [iFrame "#"|]; iClear "Hvalid_chain"; iIntros (new_info); iNamed 1.
+  wp_apply wp_NewMap; iIntros (ptr_new_updates) "Hown_new_updates".
+  wp_storeField.
+  wp_loadField.
+  wp_apply (release_spec with "[-HΦ]").
+  {
+    iFrame "HmuR Hlocked ∗#%".
+    iSplit.
+    - iPureIntro. rewrite app_length. lia.
+    - eauto.
+  }
+  wp_pures. by iApply "HΦ".
+Qed.
 
 End proofs.
